removed partial proof

misc_memory.v
@@ -6,30 +6,21 @@ Require Import List.
 Import ListNotations.
 
 
-Fixpoint word_to_bytes {size : nat} : word size -> option (list (word 8)) :=
+Fixpoint word_to_bytes (size : nat) : word size -> option (list (word 8)) :=
   match size with
   | O => fun w => Some []
   | S (S (S (S (S (S (S (S size'))))))) =>
-      fun w => match (word_to_bytes (split2 8 size' w)) with
+      fun w => match (word_to_bytes size' (split2 8 size' w)) with
                | Some l => Some ((split1 8 size' w)::l)
                | None => None
                end
   | _ => fun w => None
   end.
 
-Definition x := natToWord 16 1.
-Definition y := natToWord 15 1.
-
-Compute (word_to_bytes x).
-Compute (word_to_bytes y).
-
-
-
 Fixpoint bytes_to_word (size : nat) : list (word 8) -> option (word size) :=
   match size with
-  | O => fun l =>
-         fun l => match l with
-                  | [] => Some (wzero 0)
+  | O => fun l => match l with
+                  | [] => Some (natToWord 0 0)
                   | _ => None
                   end
   | S (S (S (S (S (S (S (S size'))))))) =>
@@ -37,9 +28,22 @@ Fixpoint bytes_to_word (size : nat) : list (word 8) -> option (word size) :=
                | [] => None
                | x::xs => match (bytes_to_word size' xs) with
                           | None => None
-                          | Some w => bbv.Word.combine x w
+                          | Some w => Some (bbv.Word.combine x w)
                           end
                end
   | _ => fun l => None
   end.
+
+
+Definition x := natToWord 16 1.
+Definition y := natToWord 15 1.
+
+
+Check word 0.
+
+Theorem word_to_bytes_bytes_to_word:
+  forall (size : nat) (w : word size) (l : list (word 8)), 
+    word_to_bytes size w = Some l -> bytes_to_word size l = Some w.
+Admitted.                    
+    
 
